src/provability.lean
@@ -4,63 +4,347 @@ universe u
 
 namespace classical_logic
 
-def mk' (F : Sort*) [has_negation F] [has_arrow F] [has_top F] [has_turnstile (set F) F]
-(deduction' : ∀ {T : set F} {p q : F}, T +{ p } ⊢ q → T ⊢ p ⟶ q)
-(weakening : ∀ {T : set F} {U : set F} {p : F}, T ⊆ U → T ⊢ p → U ⊢ p)
-(modus_ponens : ∀ {T : set F} {p q : F}, T ⊢ p ⟶ q → T ⊢ p → T ⊢ q)
-(by_axiom : ∀ {T : set F} {p : F}, p ∈ T → T ⊢ p)
-(imply₁ : ∀ {T : set F} {p q : F}, T ⊢ p ⟶ q ⟶ p)
-(imply₂ : ∀ {T : set F} {p q r : F}, T ⊢ (p ⟶ q ⟶ r) ⟶ (p ⟶ q) ⟶ p ⟶ r)
-(contrapose : ∀ {T : set F} {p q : F}, T ⊢ (⁻p ⟶ ⁻q) ⟶ q ⟶ p)
-(provable_top : ∀ {T : set F}, T ⊢ (⊤ : F)) : classical_logic (F : Sort*) :=
-{ deduction' := @deduction',
-  weakening := @weakening,
-  modus_ponens := @modus_ponens,
-  by_axiom := @by_axiom,
-  imply₁ := @imply₁,
-  imply₂ := @imply₂,
-  contrapose := @contrapose,
-  provable_top := @provable_top,
-  bot := ⁻⊤,
-  inf := λ p q, ⁻(p ⟶ ⁻q),
-  sup := λ p q, ⁻p ⟶ q,
-  provable_bot := by simp,  
-  and_def := by simp,
-  or_def := by simp }
+variables {F : Type*} [propositional_formula F] (P : set F) (T : set F) [CL : classical_logic P]
+include CL
 
-variables {F : Type*} (T : set F) [classical_logic F]
+@[simp] lemma neg_top_eq : (⁻⊤ : F) = ⊥ := eq.symm (bot_eq P)
 
-@[simp] lemma not_top_eq_bot : (⁻⊤ : F) = ⊥ := by simp[classical_logic.provable_bot]
+variables {P}
 
-@[simp] lemma refl (p : F) : T ⊢ p ⟶ p :=
+@[simp] lemma not_top_eq_bot : (⁻⊤ : F) = ⊥ := eq.symm (classical_logic.bot_eq P)
+
+local infixl ` ⨀ `:90 := modus_ponens
+
+@[simp] lemma refl (p : F) : p ⟶ p ∈ P :=
 begin
-  have l₀ : T ⊢ (p ⟶ (p ⟶ p) ⟶ p) ⟶ (p ⟶ p ⟶ p) ⟶ p ⟶ p, simp,
-  have l₁ : T ⊢ p ⟶ (p ⟶ p) ⟶ p, simp,
-  have l₂ : T ⊢ (p ⟶ p ⟶ p) ⟶ p ⟶ p, refine modus_ponens l₀ l₁,
-  have l₃ : T ⊢ p ⟶ p ⟶ p, simp,
-  refine modus_ponens l₂ l₃
+  have l₀ : (p ⟶ (p ⟶ p) ⟶ p) ⟶ (p ⟶ p ⟶ p) ⟶ p ⟶ p ∈ P, simp,
+  have l₁ : p ⟶ (p ⟶ p) ⟶ p ∈ P, simp,
+  have l₂ : (p ⟶ p ⟶ p) ⟶ p ⟶ p ∈ P, refine l₀ ⨀ l₁,
+  have l₃ : p ⟶ p ⟶ p ∈ P, simp,
+  simp[set.mem_def],
+  refine l₂ ⨀ l₃
 end
 
 variables {T}
 
-@[simp] lemma insert (p) : T+{p} ⊢ p :=
+@[simp] lemma hyp_right {p : F} (h : p ∈ P) (q) : q ⟶ p ∈ P :=
+by { have : p ⟶ q ⟶ p ∈ P, simp, exact this ⨀ h }
+
+lemma modus_ponens_hyp {p q r : F} (hqr : p ⟶ q ⟶ r ∈ P) (hq : p ⟶ q ∈ P) : p ⟶ r ∈ P :=
+by { have : (p ⟶ q ⟶ r) ⟶ (p ⟶ q) ⟶ p ⟶ r ∈ P, simp, exact this ⨀ hqr ⨀ hq }
+
+local infixl ` ⨀₁ `:90 := modus_ponens_hyp
+
+lemma modus_ponens_hyp₂ {p q r s : F} (hqr : p ⟶ q ⟶ r ⟶ s ∈ P) (hq : p ⟶ q ⟶ r ∈ P) : p ⟶ q ⟶ s ∈ P :=
+by { have : p ⟶ (q ⟶ r ⟶ s) ⟶ (q ⟶ r) ⟶ q ⟶ s ∈ P, simp, exact this ⨀₁ hqr ⨀₁ hq }
+
+local infixl ` ⨀₂ `:90 := modus_ponens_hyp₂
+
+lemma modus_ponens_hyp₃ {p q r s t : F} (hqr : p ⟶ q ⟶ r ⟶ s ⟶ t ∈ P) (hq : p ⟶ q ⟶ r ⟶ s ∈ P) : p ⟶ q ⟶ r ⟶ t ∈ P :=
+by { have : p ⟶ q ⟶ (r ⟶ s ⟶ t) ⟶ (r ⟶ s) ⟶ r ⟶ t ∈ P, simp, exact this ⨀₂ hqr ⨀₂ hq }
+
+local infixl ` ⨀₃ `:90 := modus_ponens_hyp₃
+
+lemma impl_trans {p q r : F} : (p ⟶ q ∈ P) → (q ⟶ r ∈ P) → (p ⟶ r ∈ P) := λ h₁ h₂,
+begin
+  have l₁ : (p ⟶ q ⟶ r) ⟶ (p ⟶ q) ⟶ (p ⟶ r) ∈ P, simp,  
+  have l₂ : (p ⟶ q ⟶ r) ∈ P, simp[h₂],
+  have l₃ : (p ⟶ q) ⟶ (p ⟶ r) ∈ P, from l₁ ⨀ l₂,
+  exact l₃ ⨀ h₁
+end
+
+@[simp] lemma dne (p : F) : ⁻⁻p ⟶ p ∈ P :=
+begin
+  have lmm₁ : ⁻⁻p ⟶ (⁻⁻⁻⁻p ⟶ ⁻⁻p) ⟶ ⁻p ⟶ ⁻⁻⁻p ∈ P, simp,
+  have lmm₂ : ⁻⁻p ⟶ ⁻⁻⁻⁻p ⟶ ⁻⁻p ∈ P, simp,
+  have lmm₃ : ⁻⁻p ⟶ (⁻p ⟶ ⁻⁻⁻p) ⟶ ⁻⁻p ⟶ p ∈ P, simp,  
+  have lmm₄ : ⁻⁻p ⟶ ⁻p ⟶ ⁻⁻⁻p ∈ P, from lmm₁ ⨀₁ lmm₂,
+  have lmm₅ : ⁻⁻p ⟶ ⁻⁻p ⟶ p ∈ P, from lmm₃ ⨀₁ lmm₄,
+  have lmm₆ : ⁻⁻p ⟶ ⁻⁻p ∈ P, simp,
+  exact lmm₅ ⨀₁ lmm₆
+end
+
+@[simp] lemma dni (p : F) : p ⟶ ⁻⁻p ∈ P :=
+by { have : (⁻⁻⁻p ⟶ ⁻p) ⟶ p ⟶ ⁻⁻p ∈ P, simp, exact this ⨀ (by simp) }
+
+@[simp] lemma dn_iff {p : F} : ⁻⁻p ∈ P ↔ p ∈ P :=
+⟨λ h, (show ⁻⁻p ⟶ p ∈ P, by simp) ⨀ h, λ h, (show p ⟶ ⁻⁻p ∈ P, by simp) ⨀ h⟩
+
+@[simp] lemma dn1_iff {p q : F} : (⁻⁻p ⟶ q ∈ P) ↔ (p ⟶ q ∈ P) :=
+⟨impl_trans (dni _), impl_trans (dne _)⟩
+
+@[simp] lemma dn2_iff {p q : F} : (p ⟶ ⁻⁻q ∈ P) ↔ (p ⟶ q ∈ P) :=
+⟨λ h, impl_trans h (dne _), λ h, impl_trans h (dni _)⟩
+
+lemma explosion {p : F} (h₁ : p ∈ P) (h₂ : ⁻p ∈ P) {q : F} : q ∈ P :=
+begin
+  have : ⁻p ⟶ ⁻q ⟶ ⁻p ∈ P, simp,
+  have : ⁻q ⟶ ⁻p ∈ P, from this ⨀ h₂,
+  have : p ⟶ q ∈ P, from (show (⁻q ⟶ ⁻p) ⟶ p ⟶ q ∈ P, by simp) ⨀ this,
+  exact this ⨀ h₁
+end
+
+lemma explosion_hyp {p q : F} (h₁ : p ⟶ q ∈ P) (h₂ : p ⟶ ⁻q ∈ P) {r : F} : p ⟶ r ∈ P :=
+begin
+  have : p ⟶ ⁻q ⟶ ⁻r ⟶ ⁻q ∈ P, simp,
+  have : p ⟶ ⁻r ⟶ ⁻q ∈ P, from this ⨀₁ h₂,
+  have : p ⟶ q ⟶ r ∈ P, from (show p ⟶ (⁻r ⟶ ⁻q) ⟶ q ⟶ r ∈ P, by simp) ⨀₁ this,
+  exact this ⨀₁ h₁
+end
+
+lemma explosion_hyp₂ {p q r : F} (h₁ : p ⟶ q ⟶ r ∈ P) (h₂ : p ⟶ q ⟶ ⁻r ∈ P) {s : F} : p ⟶ q ⟶ s ∈ P :=
+begin
+  have : p ⟶ q ⟶ ⁻r ⟶ ⁻s ⟶ ⁻r ∈ P, simp,
+  have : p ⟶ q ⟶ ⁻s ⟶ ⁻r ∈ P, from this ⨀₂ h₂,
+  have : p ⟶ q ⟶ r ⟶ s ∈ P, from (show p ⟶ q ⟶ (⁻s ⟶ ⁻r) ⟶ r ⟶ s ∈ P, by simp) ⨀₂ this,
+  exact this ⨀₂ h₁
+end
+
+@[simp] lemma hyp_bot {p : F} : ⊥ ⟶ p ∈ P :=
+explosion_hyp (show (⊥ ⟶ ⊤ : F) ∈ P, by simp) (show (⊥ : F) ⟶ ⁻⊤ ∈ P, by simp[neg_top_eq P])
+
+lemma contrapose {p q : F} : (⁻p ⟶ ⁻q ∈ P) ↔ (q ⟶ p ∈ P) :=
+⟨λ h, (show (⁻p ⟶ ⁻q) ⟶ q ⟶ p ∈ P, by simp) ⨀ h, λ h,
+  by { have : ⁻⁻q ⟶ p ∈ P, from impl_trans (show ⁻⁻q ⟶ q ∈ P, by simp) h,
+       exact (show (⁻⁻q ⟶ ⁻⁻p) ⟶ ⁻p ⟶ ⁻q ∈ P, by simp) ⨀ (impl_trans this (show p ⟶ ⁻⁻p ∈ P, by simp)) }⟩
+
+lemma neg_hyp {p : F} (h : p ⟶ ⁻p ∈ P) : ⁻p ∈ P :=
+begin
+  have : p ⟶ ⁻(p ⟶ ⁻p) ∈ P,
+  { have lmm₁ : p ⟶ p ∈ P, { simp }, exact explosion_hyp lmm₁ h },
+  have : (p ⟶ ⁻p) ⟶ ⁻p ∈ P, from impl_trans (dni _) (contrapose.mpr this),
+  exact this ⨀ h
+end
+
+lemma raa {p : F} (q : F) (h₁ : p ⟶ q ∈ P) (h₂ : p ⟶ ⁻q ∈ P) : ⁻p ∈ P :=
+neg_hyp (explosion_hyp h₁ h₂)
+
+@[simp] lemma and_left (p q : F) : p ⊓ q ⟶ p ∈ P :=
+begin
+  simp[and_def P],
+  have : ⁻p ⟶ p ⟶ ⁻q ∈ P, from explosion_hyp₂ (show ⁻p ⟶ p ⟶ p ∈ P, by simp) (show ⁻p ⟶ p ⟶ ⁻p ∈ P, by simp),
+  have : ⁻(p ⟶ ⁻q) ⟶ ⁻⁻p ∈ P, from contrapose.mpr this,
+  simp* at*
+end
+
+@[simp] lemma and_right (p q : F) : p ⊓ q ⟶ q ∈ P :=
+begin
+  simp[and_def P],
+  have : ⁻q ⟶ p ⟶ ⁻q ∈ P, simp,
+  have : ⁻(p ⟶ ⁻q) ⟶ q ∈ P, from impl_trans (contrapose.mpr this) (by simp),
+  exact this
+end
+
+lemma iff_and {p q : F} : (p ⊓ q ∈ P) ↔ (p ∈ P ∧ q ∈ P) :=
+⟨λ h, by { split,
+   { exact modus_ponens (show p ⊓ q ⟶ p ∈ P, by simp) h },
+   { exact modus_ponens (show p ⊓ q ⟶ q ∈ P, by simp) h } },
+ λ h, by { simp[and_def P], rcases h with ⟨h₁, h₂⟩,
+   have : (p ⟶ ⁻q) ⟶ ⁻q ∈ P, from (show (p ⟶ ⁻q) ⟶ p ⟶ ⁻q ∈ P, by simp) ⨀₁ (by simp[h₁]),
+   have : q ⟶ ⁻(p ⟶ ⁻q) ∈ P, from impl_trans (dni _) (contrapose.mpr this),
+   exact modus_ponens this h₂ }⟩
+
+lemma iff_equiv {p q : F} : (p ⟷ q ∈ P) ↔ (p ⟶ q ∈ P ∧ q ⟶ p ∈ P) :=
+by simp[lrarrow_def, iff_and]
+
+lemma equiv_imply_of_equiv {p₁ q₁ p₂ q₂ : F} (hp : p₁ ⟷ p₂ ∈ P) (hq : q₁ ⟷ q₂ ∈ P) : (p₁ ⟶ q₁) ⟷ (p₂ ⟶ q₂) ∈ P :=
+begin
+  simp[iff_equiv] at*, split,
+  { have : (p₁ ⟶ q₁) ⟶ p₂ ⟶ q₁ ∈ P, from (show (p₁ ⟶ q₁) ⟶ p₂ ⟶ p₁ ⟶ q₁ ∈ P, by simp) ⨀₂ (by simp[hp]),
+    exact (show (p₁ ⟶ q₁) ⟶ p₂ ⟶ q₁ ⟶ q₂ ∈ P, by simp[hq]) ⨀₂ this },
+  { have : (p₂ ⟶ q₂) ⟶ p₁ ⟶ q₂ ∈ P, from (show (p₂ ⟶ q₂) ⟶ p₁ ⟶ p₂ ⟶ q₂ ∈ P, by simp) ⨀₂ (by simp[hp]),
+    exact (show (p₂ ⟶ q₂) ⟶ p₁ ⟶ q₂ ⟶ q₁ ∈ P, by simp[hq]) ⨀₂ this }
+end
+
+lemma imply_of_equiv {p₁ q₁ p₂ q₂ : F} (h : p₁ ⟶ q₁ ∈ P) (hp : p₁ ⟷ p₂ ∈ P) (hq : q₁ ⟷ q₂ ∈ P) : p₂ ⟶ q₂ ∈ P :=
+by { have : (p₁ ⟶ q₁) ⟶ p₂ ⟶ q₂ ∈ P ∧ (p₂ ⟶ q₂) ⟶ p₁ ⟶ q₁ ∈ P, from iff_equiv.mp (equiv_imply_of_equiv hp hq),
+     exact this.1 ⨀ h }
+
+lemma equiv_neg_of_equiv {p₁ p₂ : F} (hp : p₁ ⟷ p₂ ∈ P) : ⁻p₁ ⟷ ⁻p₂ ∈ P :=
+by simp[iff_equiv, contrapose] at*; simp[hp]
+
+lemma neg_of_equiv {p₁ p₂ : F} (h : ⁻p₁ ∈ P) (hp : p₁ ⟷ p₂ ∈ P) : ⁻p₂ ∈ P :=
+by { have : ⁻p₁ ⟶ ⁻p₂ ∈ P, from (iff_equiv.mp (equiv_neg_of_equiv hp)).1, exact this ⨀ h }
+
+lemma equiv_and_of_equiv {p₁ q₁ p₂ q₂: F} (hp : p₁ ⟷ p₂ ∈ P) (hq : q₁ ⟷ q₂ ∈ P) : p₁ ⊓ q₁ ⟷ p₂ ⊓ q₂ ∈ P :=
+by { simp[and_def P], refine equiv_neg_of_equiv (equiv_imply_of_equiv hp (equiv_neg_of_equiv hq)) }
+
+lemma and_of_equiv {p₁ q₁ p₂ q₂: F} (h : p₁ ⊓ q₁ ∈ P) (hp : p₁ ⟷ p₂ ∈ P) (hq : q₁ ⟷ q₂ ∈ P) : p₂ ⊓ q₂ ∈ P :=
+by { have : p₁ ⊓ q₁ ⟶ p₂ ⊓ q₂ ∈ P, from (iff_equiv.mp (equiv_and_of_equiv hp hq)).1, exact this ⨀ h }
+
+lemma equiv_or_of_equiv {p₁ q₁ p₂ q₂: F} (hp : p₁ ⟷ p₂ ∈ P) (hq : q₁ ⟷ q₂ ∈ P) : p₁ ⊔ q₁ ⟷ p₂ ⊔ q₂ ∈ P :=
+by { simp[or_def P], refine (equiv_imply_of_equiv (equiv_neg_of_equiv hp) hq) }
+
+lemma or_of_equiv {p₁ q₁ p₂ q₂: F} (h : p₁ ⊔ q₁ ∈ P) (hp : p₁ ⟷ p₂ ∈ P) (hq : q₁ ⟷ q₂ ∈ P) : p₂ ⊔ q₂ ∈ P :=
+by { have : p₁ ⊔ q₁ ⟶ p₂ ⊔ q₂ ∈ P, from (iff_equiv.mp (equiv_or_of_equiv hp hq)).1, exact this ⨀ h }
+
+lemma equiv_equiv_of_equiv {p₁ q₁ p₂ q₂: F} (hp : p₁ ⟷ p₂ ∈ P) (hq : q₁ ⟷ q₂ ∈ P) : (p₁ ⟷ q₁) ⟷ (p₂ ⟷ q₂) ∈ P :=
+by { refine (equiv_and_of_equiv (equiv_imply_of_equiv hp hq) (equiv_imply_of_equiv hq hp)) }
+
+lemma equiv_of_equiv {p₁ q₁ p₂ q₂: F} (h : p₁ ⟷ q₁ ∈ P) (hp : p₁ ⟷ p₂ ∈ P) (hq : q₁ ⟷ q₂ ∈ P) : p₂ ⟷ q₂ ∈ P :=
+by { have : (p₁ ⟷ q₁) ⟶ (p₂ ⟷ q₂) ∈ P, from (iff_equiv.mp (equiv_equiv_of_equiv hp hq)).1, exact this ⨀ h }
+
+@[simp] lemma equiv_refl (p : F) : p ⟷ p ∈ P := by simp[iff_equiv]
+
+lemma equiv_symm {p q : F} : p ⟷ q ∈ P → q ⟷ p ∈ P := by { simp[iff_equiv], intros, simp* }
+
+lemma equiv_trans {p q r : F} : p ⟷ q ∈ P → q ⟷ r ∈ P → p ⟷ r ∈ P :=
+by { simp[iff_equiv], intros hpq hqp hqr hrq, exact ⟨impl_trans hpq hqr, impl_trans hrq hqp⟩ }
+
+
+variables (P)
+
+@[reducible] def equiv (p q : F) : Prop := p ⟷ q ∈ P
+
+theorem equiv_equivalence : equivalence (equiv P) :=
+⟨equiv_refl, @equiv_symm _ _ _ _, @equiv_trans _ _ _ _⟩
+
+variables {P}
+
+@[simp] lemma iff_dn_refl_right {p : F} : p ⟷ ⁻⁻p ∈ P := by simp[iff_equiv]
+
+@[simp] lemma iff_dn_refl_left {p : F} : ⁻⁻p ⟷ p ∈ P := by simp[iff_equiv]
+
+@[simp] lemma contraposition_inv {p q : F} : (p ⟶ q) ⟶ (⁻q ⟶ ⁻p) ∈ P :=
+by { have : (⁻⁻p ⟶ ⁻⁻q) ⟶ ⁻q ⟶ ⁻p ∈ P, simp, 
+     refine imply_of_equiv this (equiv_imply_of_equiv _ _) _; simp }
+
+@[simp] lemma contraposition_iff {p q : F} : (p ⟶ q) ⟷ (⁻q ⟶ ⁻p) ∈ P :=
+by simp[iff_equiv]
+
+@[simp] lemma contraposition_iff_inv {p q : F} : (⁻q ⟶ ⁻p) ⟷ (p ⟶ q) ∈ P :=
+by simp[iff_equiv]
+
+@[simp] lemma neg_hyp' {p : F} : (p ⟶ ⁻p) ⟶ ⁻p ∈ P :=
+begin
+  have : (p ⟶ ⁻p) ⟶ p ⟶ ⁻(p ⟶ ⁻p) ∈ P,
+  { have lmm₁ : (p ⟶ ⁻p) ⟶ p ⟶ p ∈ P, { simp }, exact explosion_hyp₂ lmm₁ (by simp) },
+  have : (p ⟶ ⁻p) ⟶ ⁻⁻(p ⟶ ⁻p) ⟶ ⁻p ∈ P,
+  { refine imply_of_equiv this _ _; simp[iff_equiv] },
+  exact this ⨀₁ (show (p ⟶ ⁻p) ⟶ ⁻⁻(p ⟶ ⁻p) ∈ P, by simp)
+end
+
+@[simp] lemma neg_iff (p : F) : ⁻p ⟷ (p ⟶ ⊥) ∈ P :=
+begin
+  simp[iff_equiv], split,
+  { exact explosion_hyp₂ (show ⁻p ⟶ p ⟶ p ∈ P, by simp) (show ⁻p ⟶ p ⟶ ⁻p ∈ P, by simp) },
+  { have : (p ⟶ ⊥) ⟶ p ⟶ ⁻p ∈ P,
+      from explosion_hyp₂ (show (p ⟶ ⊥) ⟶ p ⟶ ⊤ ∈ P, by simp) (show (p ⟶ ⊥) ⟶ p ⟶ ⁻⊤ ∈ P, by simp[bot_eq P]),
+    refine (show (p ⟶ ⊥) ⟶ (p ⟶ ⁻p) ⟶ ⁻p ∈ P, by simp) ⨀₁ this }
+end
+
+@[simp] lemma neg_imp {p q : F} : ⁻(p ⟶ q) ⟷ p ⊓ ⁻q ∈ P :=
+by simp [and_def P]; refine (equiv_neg_of_equiv (equiv_imply_of_equiv _ _)); simp
+
+@[simp] lemma neg_imp' {p q : F} : (⁻(p ⟶ q) ∈ P) ↔ (p ⊓ ⁻q ∈ P) :=
+begin
+  simp [and_def P], split; intros h,
+  { refine neg_of_equiv h (equiv_imply_of_equiv _ _); simp },
+  { refine neg_of_equiv h (equiv_imply_of_equiv _ _); simp }
+end
+
+@[simp] lemma equiv_symm_and (p q : F) : p ⊓ q ⟷ q ⊓ p ∈ P :=
+by { simp only [and_def P], refine equiv_neg_of_equiv _,
+     refine equiv_of_equiv (show p ⟶ ⁻q ⟷ ⁻⁻q ⟶ ⁻p ∈ P, by simp) _ (equiv_imply_of_equiv _ _); simp }
+
+@[simp] lemma equiv_symm_equiv (p q : F) : (p ⟷ q) ⟷ (q ⟷ p) ∈ P := equiv_symm_and _ _
+
+@[simp] lemma equiv_symm_or (p q : F) : p ⊔ q ⟷ q ⊔ p ∈ P :=
+by { simp [or_def P],
+     refine equiv_of_equiv (show ⁻p ⟶ q ⟷ ⁻q ⟶ ⁻⁻p ∈ P, by simp) _ (equiv_imply_of_equiv _ _); simp }
+
+@[simp] lemma and_destruct {p q : F} : p ⟶ q ⟶ p ⊓ q ∈ P :=
+by { simp only [and_def P],
+     have : p ⟶ (p ⟶ ⁻q) ⟶ ⁻q ∈ P, from (show p ⟶ (p ⟶ ⁻q) ⟶ p ⟶ ⁻q ∈ P, by simp) ⨀₂ (show p ⟶ (p ⟶ ⁻q) ⟶ p ∈ P, by simp),
+     refine imply_of_equiv this (by simp) _,
+     have : (p ⟶ ⁻q) ⟶ ⁻q ⟷ ⁻⁻q ⟶ ⁻(p ⟶ ⁻q) ∈ P, { simp }, refine equiv_of_equiv this _ (equiv_imply_of_equiv _ _); simp }
+
+@[simp] lemma imply_or_left (p q : F) : p ⟶ p ⊔ q ∈ P :=
+by simp[or_def P]; refine explosion_hyp₂ (show p ⟶ ⁻p ⟶ p ∈ P, by simp) (show p ⟶ ⁻p ⟶ ⁻p ∈ P, by simp)
+
+@[simp] lemma imply_or_right (p q : F) : q ⟶ p ⊔ q ∈ P :=
+by simp[or_def P]
+
+@[simp] lemma imply_and {p q r : F} : (p ⟶ q) ⟶ (p ⟶ r) ⟶ p ⟶ q ⊓ r ∈ P :=
+begin
+  have : (p ⟶ q) ⟶ (p ⟶ r) ⟶ p ⟶ r ⟶ q ⊓ r ∈ P,
+    from (show (p ⟶ q) ⟶ (p ⟶ r) ⟶ p ⟶ q ⟶ r ⟶ q ⊓ r ∈ P, by simp) ⨀₃ (show (p ⟶ q) ⟶ (p ⟶ r) ⟶ p ⟶ q ∈ P, by simp),
+  exact this ⨀₃ (show (p ⟶ q) ⟶ (p ⟶ r) ⟶ p ⟶ r ∈ P, by simp),
+end
+
+@[simp] lemma neg_and_equiv_or_neg {p q : F} : ⁻(p ⊓ q) ⟷ ⁻p ⊔ ⁻q ∈ P :=
+begin
+  simp [and_def P, or_def P],
+  refine equiv_of_equiv (show p ⟶ ⁻q ⟷ p ⟶ ⁻q ∈ P, by simp) _ (equiv_imply_of_equiv _ _); simp
+end
+
+@[simp] lemma neg_or_equiv_and_neg {p q : F} : ⁻(p ⊔ q) ⟷ ⁻p ⊓ ⁻q ∈ P :=
+begin
+  simp [and_def P, or_def P],
+  refine equiv_of_equiv (show ⁻(⁻p ⟶ q) ⟷ ⁻(⁻p ⟶ q) ∈ P, by simp) _ (equiv_neg_of_equiv (equiv_imply_of_equiv _ _)); simp
+end
+
+@[simp] lemma hyp_or {p q r : F} : (p ⟶ r) ⟶ (q ⟶ r) ⟶ p ⊔ q ⟶ r ∈ P :=
+begin
+  have : (⁻r ⟶ ⁻p) ⟶ (⁻r ⟶ ⁻q) ⟶ ⁻r ⟶ ⁻p ⊓ ⁻q ∈ P, { simp },
+  refine imply_of_equiv this (by simp) (equiv_imply_of_equiv (by simp) _),
+  have : ⁻r ⟶ ⁻(p ⊔ q) ⟷ p ⊔ q ⟶ r ∈ P, { simp },
+  refine equiv_of_equiv (show ⁻r ⟶ ⁻(p ⊔ q) ⟷ p ⊔ q ⟶ r ∈ P, by simp) (equiv_imply_of_equiv _ _) _; simp
+end
+
+variables (P)
+
+def lindenbaum := quotient (⟨equiv P, equiv_equivalence P⟩ : setoid F)
+
+
+
+end classical_logic
+
+namespace axiomatic_classical_logic
+open classical_logic
+variables {F : Type*} [propositional_formula F] (T : set F) [axiomatic_classical_logic F]
+
+instance : classical_logic ((⊢) T) := axiomatic_classical_logic.classical
+
+
+variables {T}
+
+lemma modus_ponens {p q : F} : T ⊢ p ⟶ q → T ⊢ p → T ⊢ q := modus_ponens
+
+local infixr ` ⨀ `:90 := axiomatic_classical_logic.modus_ponens
+
+@[simp] lemma imply₁ (p q) : T ⊢ p ⟶ q ⟶ p := imply₁
+
+@[simp] lemma imply₂ (p q r) : T ⊢ (p ⟶ q ⟶ r) ⟶ (p ⟶ q) ⟶ p ⟶ r := imply₂
+
+@[simp] lemma contraposition (p q) : T ⊢ (⁻p ⟶ ⁻q) ⟶ q ⟶ p := contraposition
+
+@[simp] lemma provable_top : T ⊢ (⊤ : F) := provable_top
+
+@[simp] lemma dne (p : F) : T ⊢ ⁻⁻p ⟶ p := dne p
+
+@[simp] lemma dni (p : F) : T ⊢ p ⟶ ⁻⁻p := dni p
+
+
+
+@[simp] lemma insert (p) : T +{ p } ⊢ p :=
 by_axiom (by simp)
 
 @[simp] lemma weakening_insert {q : F} (h : T ⊢ q) (p) : T +{ p } ⊢ q :=
 weakening (show T ⊆ T +{ p }, by { intros x h, simp[h] }) h
 
 theorem deduction {p q} : (T +{ p } ⊢ q) ↔ (T ⊢ p ⟶ q) :=
-⟨deduction', λ h, by { have : T+{p} ⊢ p ⟶ q, simp[h], exact modus_ponens this (by simp) }⟩
+⟨deduction', λ h, by { have : T +{ p } ⊢ p ⟶ q, simp[h], exact this ⨀ (by simp) }⟩
 
-@[simp] lemma hyp_right {p : F} (h : T ⊢ p) (q) : T ⊢ q ⟶ p :=
-by { have : T ⊢ p ⟶ q ⟶ p, simp,
-     exact modus_ponens this h }
+@[simp] lemma refl (p : F) : T ⊢ p ⟶ p := classical_logic.refl p
+
+@[simp] lemma hyp_right {p : F} (h : T ⊢ p) (q) : T ⊢ q ⟶ p := hyp_right h q
 
 lemma modus_ponens_hyp {p q r: F} (hqr : T ⊢ p ⟶ q ⟶ r) (hq : T ⊢ p ⟶ q) : T ⊢ p ⟶ r :=
 by { have : T ⊢ (p ⟶ q ⟶ r) ⟶ (p ⟶ q) ⟶ p ⟶ r, simp,
      exact modus_ponens (modus_ponens this hqr) hq }
 
-lemma imp_trans {p q r : F} : (T ⊢ p ⟶ q) → (T ⊢ q ⟶ r) → (T ⊢ p ⟶ r) := λ h₁ h₂,
+lemma impl_trans {p q r : F} : (T ⊢ p ⟶ q) → (T ⊢ q ⟶ r) → (T ⊢ p ⟶ r) := λ h₁ h₂,
 begin
   have l₁ : T ⊢ (p ⟶ q ⟶ r) ⟶ (p ⟶ q) ⟶ (p ⟶ r), simp,  
   have l₂ : T ⊢ (p ⟶ q ⟶ r), simp[h₂],
@@ -68,143 +352,17 @@ begin
   exact modus_ponens l₃ h₁
 end
 
-@[simp] lemma dne (p : F) : T ⊢ ⁻⁻p ⟶ p :=
-begin
-  have lmm₁ : T ⊢ ⁻⁻p ⟶ (⁻⁻⁻⁻p ⟶ ⁻⁻p) ⟶ ⁻p ⟶ ⁻⁻⁻p, simp,
-  have lmm₂ : T ⊢ ⁻⁻p ⟶ ⁻⁻⁻⁻p ⟶ ⁻⁻p, simp,
-  have lmm₃ : T ⊢ ⁻⁻p ⟶ (⁻p ⟶ ⁻⁻⁻p) ⟶ ⁻⁻p ⟶ p, simp,  
-  have lmm₄ : T ⊢ ⁻⁻p ⟶ ⁻p ⟶ ⁻⁻⁻p, from modus_ponens_hyp lmm₁ lmm₂,
-  have lmm₅ : T ⊢ ⁻⁻p ⟶ ⁻⁻p ⟶ p, from modus_ponens_hyp lmm₃ lmm₄,
-  have lmm₆ : T ⊢ ⁻⁻p ⟶ ⁻⁻p, simp,
-  exact modus_ponens_hyp lmm₅ lmm₆
-end
 
-@[simp] lemma dni (p : F) : T ⊢ p ⟶ ⁻⁻p :=
-by { have : T ⊢ (⁻⁻⁻p ⟶ ⁻p) ⟶ p ⟶ ⁻⁻p, simp,
-     exact modus_ponens this (by simp) }
-
-@[simp] lemma dn_iff {p : F} : T ⊢ ⁻⁻p ↔ T ⊢ p :=
-⟨λ h, modus_ponens (show T ⊢ ⁻⁻p ⟶ p, by simp) h, λ h, modus_ponens (show T ⊢ p ⟶ ⁻⁻p, by simp) h⟩
-
-
-@[simp] lemma dn1_iff {p q : F} : (T ⊢ ⁻⁻p ⟶ q) ↔ (T ⊢ p ⟶ q) :=
-⟨imp_trans (dni _), imp_trans (dne _)⟩
-
-@[simp] lemma dn2_iff {p q : F} : (T ⊢ p ⟶ ⁻⁻q) ↔ (T ⊢ p ⟶ q) :=
-⟨λ h, imp_trans h (dne _), λ h, imp_trans h (dni _)⟩
-
-lemma explosion {p : F} (h₁ : T ⊢ p) (h₂ : T ⊢ ⁻p) {q : F} : T ⊢ q :=
-begin
-  have : T ⊢ ⁻p ⟶ ⁻q ⟶ ⁻p, simp,
-  have : T ⊢ ⁻q ⟶ ⁻p, from modus_ponens this h₂,
-  have : T ⊢ p ⟶ q, from modus_ponens (show T ⊢ (⁻q ⟶ ⁻p) ⟶ p ⟶ q, by simp) this,
-  exact modus_ponens this h₁
-end
-
-lemma explosion_hyp {p q : F} (h₁ : T ⊢ p ⟶ q) (h₂ : T ⊢ p ⟶ ⁻q) {r : F} : T ⊢ p ⟶ r :=
-begin
-  have : T ⊢ p ⟶ ⁻q ⟶ ⁻r ⟶ ⁻q, simp,
-  have : T ⊢ p ⟶ ⁻r ⟶ ⁻q, from modus_ponens_hyp this h₂,
-  have : T ⊢ p ⟶ q ⟶ r, from modus_ponens_hyp (show T ⊢ p ⟶ (⁻r ⟶ ⁻q) ⟶ q ⟶ r, by simp) this,
-  exact modus_ponens_hyp this h₁
-end
-
-@[simp] lemma hyp_bot {p : F} : T ⊢ ⊥ ⟶ p :=
-explosion_hyp (show T ⊢ (⊥ ⟶ ⊤ : F), by simp) (show T ⊢ (⊥ ⟶ ⁻⊤ : F), by simp)
-
-lemma contraposition {p q : F} : (T ⊢ ⁻p ⟶ ⁻q) ↔ (T ⊢ q ⟶ p) :=
-⟨λ h, modus_ponens (show T ⊢ (⁻p ⟶ ⁻q) ⟶ q ⟶ p, by simp) h, λ h,
-  by { refine modus_ponens (show T ⊢ (⁻⁻q ⟶ ⁻⁻p) ⟶ ⁻p ⟶ ⁻q, by simp) _,
-       have : T ⊢ ⁻⁻q ⟶ p, from imp_trans (show T ⊢ ⁻⁻q ⟶ q, by simp) h,
-       exact imp_trans this (show T ⊢ p ⟶ ⁻⁻p, by simp) }⟩
-
-lemma neg_hyp {p : F} (h : T ⊢ p ⟶ ⁻p) : T ⊢ ⁻p :=
-begin
-  have : T+{p} ⊢ ⁻(p ⟶ ⁻p),
-  { have lmm₁ : T+{p} ⊢ p, simp,
-    have lmm₂ : T+{p} ⊢ ⁻p, from modus_ponens (weakening_insert h _) lmm₁,
-    exact explosion lmm₁ lmm₂ },
-  have : T ⊢ p ⟶ ⁻(p ⟶ ⁻p), from deduction.mp this,
-  have : T ⊢ (p ⟶ ⁻p) ⟶ ⁻p, from imp_trans (dni _) (contraposition.mpr this),
-  exact modus_ponens this h
-end
-
-lemma raa {p : F} (q : F) (h₁ : T +{ p } ⊢ q) (h₂ : T +{ p } ⊢ ⁻q) : T ⊢ ⁻p :=
-neg_hyp (deduction.mp (explosion h₁ h₂))
-
-@[simp] lemma and_left (p q : F) : T ⊢ p ⊓ q ⟶ p :=
-begin
-  simp[and_def],
-  have : T+{⁻p}+{p} ⊢ ⁻q, 
-    from explosion (show T+{⁻p}+{p} ⊢ p, by simp) (show T+{⁻p}+{p} ⊢ ⁻p, by simp),
-  have : T ⊢ ⁻p ⟶ p ⟶ ⁻q, from (deduction.mp (deduction.mp this)),
-  exact imp_trans (contraposition.mpr this) (by simp)
-end
-
-@[simp] lemma and_right (p q : F) : T ⊢ p ⊓ q ⟶ q :=
-begin
-  simp[and_def],
-  have : T ⊢ ⁻q ⟶ p ⟶ ⁻q, simp,
-  have : T ⊢ ⁻(p ⟶ ⁻q) ⟶ q, from imp_trans (contraposition.mpr this) (by simp),
-  exact this
-end
-
-@[simp] lemma and {p q : F} : (T ⊢ p ⊓ q) ↔ (T ⊢ p ∧ T ⊢ q) :=
-⟨λ h, by { split,
-   { exact modus_ponens (show T ⊢ p ⊓ q ⟶ p, by simp) h },
-   { exact modus_ponens (show T ⊢ p ⊓ q ⟶ q, by simp) h } },
- λ h, by {simp[and_def], rcases h with ⟨h₁, h₂⟩,
-   show T ⊢ ⁻(p ⟶ ⁻q),
-   have : T+{p ⟶ ⁻q} ⊢ ⁻q, from modus_ponens (insert _) (by simp[h₁]),
-   have : T ⊢ (p ⟶ ⁻q) ⟶ ⁻q, from deduction.mp this,
-   have : T ⊢ q ⟶ ⁻(p ⟶ ⁻q), from imp_trans (dni _) (contraposition.mpr this),
-   exact modus_ponens this h₂ }⟩
-
-@[simp] lemma iff {p q : F} : (T ⊢ p ⟷ q) ↔ (T ⊢ p ⟶ q ∧ T ⊢ q ⟶ p) :=
-by simp[lrarrow_def]
-
-@[simp] lemma neg_imp {p q : F} : (T ⊢ ⁻(p ⟶ q)) ↔ (T ⊢ p ⊓ ⁻q) :=
-begin
-  simp only [and_def], split; intros h,
-  { apply raa (p ⟶ q),
-    { have : T+{p ⟶ ⁻⁻q} ⊢ p ⟶ ⁻⁻q, from insert _, simp* at * },
-    { simp[h] } },
-  { apply raa (p ⟶ ⁻⁻q); simp[h] }
-end
-
-lemma or_l (p q : F) : T ⊢ p ⟶ p ⊔ q :=
-by simp[or_def]; refine deduction.mp (deduction.mp (explosion (show T +{ p } +{ ⁻p } ⊢ p, by simp) (by simp)))
-
-lemma or_r (p q : F) : T ⊢ q ⟶ p ⊔ q :=
-by simp[or_def]; refine deduction.mp (weakening h _)
-
-lemma hyp_or {p₁ p₂ q : F} : (T ⊢ p₁ ⟶ q) → (T ⊢ p₂ ⟶ q) → (T ⊢ p₁ ⊔ p₂ ⟶ q) := λ h₁ h₂,
-begin
-  simp[or_def], apply contraposition.mp, refine deduction.mp _, simp,
-  refine ⟨deduction.mpr (contraposition.mpr h₁), deduction.mpr (contraposition.mpr h₂)⟩, 
-end
-
-lemma hyp_and_left {p₁ p₂ q : F} : (T ⊢ p₁ ⟶ q) → (T ⊢ p₁ ⊓ p₂ ⟶ q) := λ h,
-begin
-  have : T+{p₁ ⊓ p₂} ⊢ p₁, { have : T+{p₁ ⊓ p₂} ⊢ p₁ ⊓ p₂, from insert _, simp* at * },
-  refine deduction.mp (modus_ponens (show T+{p₁ ⊓ p₂} ⊢ p₁ ⟶ q, by simp[h]) this)
-end
-
-lemma hyp_and_right {p₁ p₂ q : F} : (T ⊢ p₂ ⟶ q) → (T ⊢ p₁ ⊓ p₂ ⟶ q) := λ h,
-begin
-  have : T+{p₁ ⊓ p₂} ⊢ p₂, { have : T+{p₁ ⊓ p₂} ⊢ p₁ ⊓ p₂, from insert _, simp* at * },
-  refine deduction.mp (modus_ponens (show T+{p₁ ⊓ p₂} ⊢ p₂ ⟶ q, by simp[h]) this)
-end
 
 lemma axiom_and {p₁ p₂ q : F} : T +{ p₁ ⊓ p₂ } ⊢ q ↔ T +{ p₁ } +{ p₂ } ⊢ q :=
 ⟨λ h,
- by { have lmm₁ : T+{p₁}+{p₂} ⊢ p₁ ⊓ p₂, by simp,
-      have lmm₂ : T+{p₁}+{p₂} ⊢ p₁ ⊓ p₂ ⟶ q, simp[deduction.mp h],
+ by { have lmm₁ : T +{ p₁ } +{ p₂ } ⊢ p₁ ⊓ p₂, by simp,
+      have lmm₂ : T +{ p₁ } +{ p₂ } ⊢ p₁ ⊓ p₂ ⟶ q, simp[deduction.mp h],
       exact modus_ponens lmm₂ lmm₁ },
  λ h,
- by { have lmm₁ : T+{p₁ ⊓ p₂} ⊢ p₁ ⟶ p₂ ⟶ q, simp[deduction.mp (deduction.mp h)],
-      have lmm₂ : T+{p₁ ⊓ p₂} ⊢ p₁ ⊓ p₂, from insert _, simp at lmm₂,
+ by { have lmm₁ : T +{ p₁ ⊓ p₂ } ⊢ p₁ ⟶ p₂ ⟶ q, simp[deduction.mp (deduction.mp h)],
+      have lmm₂ : T +{ p₁ ⊓ p₂ } ⊢ p₁ ⊓ p₂, from insert _, simp at lmm₂,
       exact modus_ponens (modus_ponens lmm₁ lmm₂.1) lmm₂.2 } ⟩
 
-end classical_logic
+end axiomatic_classical_logic
 
